some small Coq progress

coq/Input.v
@@ -1,5 +1,4 @@
 Require Import Coq.ZArith.BinInt.
-Require Import ListSet.
 Require Import List.
 Require Import Omega.
 Require Import Ensembles.
@@ -11,92 +10,247 @@ Require Import CpdtTactics.
 Require Import LibTactics.
 Require Import Misc.
 
+Set Implicit Arguments.
+
+Open Scope list_scope.
 
 (* * * * * * * * * * * * * * * * * * * * * * * * *)
 (*                 Definitions                   *)
 (* * * * * * * * * * * * * * * * * * * * * * * * *)
 
 Axiom V : Type.
-Definition Ty := Ensemble V.
-Definition IsA v T := In V T v.
-Definition Subtype T1 T2 := Included V T1 T2.
+Axiom V_eq_dec : forall (v1 v2: V), {v1 = v2} + {v1 <> v2}.
+Notation Ty := (Ensemble V).
+Definition IsEmpty : Ty -> Prop := Inhabited V.
+Axiom IsEmpty_dec : forall (t: Ty), {IsEmpty t} + {~ IsEmpty t}.
+Notation IsA v T := (In V T v).
+Axiom IsA_dec : forall (v:V) (t: Ty), {IsA v t} + {~ IsA v t}.
+Notation "T1 <: T2" := (Included V T1 T2) (at level 70).
+
+Definition emptyTy : Ty := Empty_set V.
+Definition anyTy : Ty := Full_set V.
+Definition tyOr : Ty -> Ty -> Ty := Union V.
+Definition tyAnd : Ty -> Ty -> Ty := Intersection V.
+Definition tyDiff : Ty -> Ty -> Ty := Setminus V.
+Definition tyNot : Ty -> Ty := tyDiff anyTy.
 
 (* A single function arrow *)
 Inductive arrow : Type :=
 | Arrow : Ty -> Ty -> arrow.
 
-(* Since an empty intersection/disjunction of arrows *)
-(* has an empty domain we can omit it WLOG so our *)
-(* proofs can focus on the interesting cases. *)
+Definition ameet (a1 a2 : arrow) : arrow :=
+  match a1, a2 with
+  | Arrow d1 r1, Arrow d2 r2 => Arrow (tyAnd d1 d2) (tyAnd r1 r2)
+  end.
 
-(* An intersection of arrows (i.e. a clause in the DNF rep)*)
-Inductive clause : Type :=
-| CBase : arrow -> clause
-| CCons : arrow -> clause -> clause.
+Definition dom (a : arrow) : Ty :=
+  match a with
+  | Arrow t1 _ => t1
+  end.
 
-(* A disjunction of intersection of arrows *)
-Inductive dnf : Type :=
-| DBase : clause -> dnf
-| DCons : clause -> dnf -> dnf.
+Definition rng (a : arrow) : Ty :=
+  match a with
+  | Arrow _ t2 => t2
+  end.
 
 Inductive res : Type :=
 | Err : res (* invalid argument/type error *)
 | Bot : res (* non-termination *)
-| Res : V -> res. (* A value result *)
+| Res : V -> res. (* a value result *)
+
+Definition fn := (V -> res).
+
+Definition FnArrow (a : arrow) (f : fn) : Prop :=
+  match a with
+  | Arrow T1 T2 =>
+    forall v,
+      (IsA v T1) ->
+      (f v = Bot \/ exists v', IsA v' T2 /\ f v = Res v')
+  end.
 
 
-Inductive  TypedArrow : (V -> res) -> arrow -> Prop :=
-| TyArrow : forall (T1 T2 : Ty) (f:(V -> res)),
-    (forall v, (~ IsA v T1) -> f v = Err) ->
-    (forall v,
-        (IsA v T1) ->
-        (f v = Bot \/ exists v', IsA v' T2 /\ f v = Res v')) ->
-    TypedArrow f (Arrow T1 T2).
+Inductive interface : Type :=
+| IBase : arrow -> interface
+| ICons : arrow -> interface -> interface.
 
 
-Inductive TypedClause : (V -> res) -> clause -> Prop :=
-| TyCBase : forall (f:(V -> res)) a,
-    TypedArrow f a ->
-    TypedClause f (CBase a)
-| TyCCons : forall (f:(V -> res)) a c,
-    TypedArrow f a ->
-    TypedClause f c ->
-    TypedClause f (CCons a c).
+Fixpoint idom (i : interface) : Ty :=
+  match i with
+  | IBase a => dom a
+  | ICons a i' => tyOr (dom a) (idom i')
+  end.
 
-Inductive TypedDNF : (V -> res) -> dnf -> Prop :=
-| TyDBase : forall (f:(V -> res)) c,
-    TypedClause f c ->
-    TypedDNF f (DBase c)
-| TyDHead : forall (f:(V -> res)) c d,
-    TypedClause f c ->
-    TypedDNF f (DCons c d)
-| TyDTail : forall (f:(V -> res)) c d,
-    TypedDNF f d ->
-    TypedDNF f (DCons c d).
 
-Inductive InputType : (V -> res) -> Ty -> Ty -> Prop :=
-| InTy :  forall (f:(V -> res)) inT outT,
-    (forall v v',
-        (f v = Res v' /\ IsA v' outT) ->
-        IsA v inT) ->
-    InputType f outT inT.
+Fixpoint FnInterface (i : interface) (f : fn) : Prop :=
+  match i with
+  | IBase a  => FnArrow a f
+  | ICons a i' => (FnArrow a f) /\ (FnInterface i' f)
+  end.
+
+
+Definition InterfaceInput
+           (i:interface)
+           (inT outT : Ty) : Prop :=
+forall (f:fn),
+  FnInterface i f ->
+  forall (v v':V),
+    IsA v (idom i) ->
+    f v = Res v' ->
+    IsA v' outT ->
+    IsA v inT.
+
+Fixpoint iapp (i1 i2 : interface) : interface :=
+  match i1 with
+  | IBase a => ICons a i2
+  | ICons a i1' => ICons a (iapp i1' i2)
+  end.
+
+Fixpoint imap (f : arrow -> arrow) (i : interface) : interface :=
+  match i with
+  | IBase a => IBase (f a)
+  | ICons a i' => ICons (f a) (imap f i')
+  end.
+
+(* non-empty subsets of an interface, as arrows with
+   pointwise intersected domain and codomains *)
+Fixpoint ipowerset (i : interface) : interface :=
+  match i with
+  | IBase a => IBase a
+  | ICons a i' => let p := ipowerset i' in
+                  iapp p (imap (ameet a) p)
+  end.
+
+Lemma interface_app : forall i i' f,
+    FnInterface i f ->
+    FnInterface i' f ->
+    FnInterface (iapp i i') f.
+Proof.
+  intro i.
+  induction i; crush.
+Qed.
+
+
+Lemma ameet_arrow_fn : forall a a' f,
+    FnArrow a f ->
+    FnArrow a' f ->
+    FnArrow (ameet a a') f.
+Proof.
+  intros a a' f. intros.
+  destruct a as [d r]. destruct a' as [d' r'].
+  simpl. intros.
+  match goal with
+  | [H : IsA _ _ |- _] => inversion H
+  end.
+  repeat
+    (match goal with
+     | [H1 : FnArrow _ _ , H2 : IsA _ _ |- _] => apply H1 in H2
+     end).
+  crush.
+  right.
+  match goal with
+  | [H : _ _ = Res ?v |- _] => exists v; rewrite H in *
+  end.
+  crush.
+  constructor; auto.
+Qed.
+  
+Lemma ameet_preserves_interface : forall i f a,
+    FnInterface i f ->
+    FnArrow a f ->
+    FnInterface (imap (ameet a) i) f.
+Proof.
+  intro i.
+  induction i as [a' | a' i']; intros.
+  simpl.
+  apply ameet_arrow_fn; crush.
+  simpl. split.
+  apply ameet_arrow_fn; crush.
+  crush.
+Qed.  
+
+Lemma ipowerset_preserves_interface : forall i i' f,
+    FnInterface i f ->
+    ipowerset i = i' ->
+    FnInterface i' f.
+Proof with crush.
+  intro i.
+  induction i...
+  assert (FnInterface (ipowerset i) f) as Hp...
+  apply interface_app...
+  apply ameet_preserves_interface...
+Qed.
+    
+    
+    
+    
+(* A disjunction of interfaces *)
+Inductive dnf : Type :=
+| DBase : interface -> dnf
+| DCons : interface -> dnf -> dnf.
+
+Fixpoint ddom (d : dnf) : Ty :=
+  match d with
+  | DBase i => idom i
+  | DCons i d' => tyAnd (idom i) (ddom d')
+  end.
+
+Fixpoint DnfFn (d : dnf) (f : fn) : Prop :=
+  match d with
+  | DBase i  => InterfaceFn i f
+  | DCons i d' => (InterfaceFn i f) \/ (DnfFn d' f)
+  end.
+
+
+Definition DnfInput
+           (d:dnf)
+           (inT outT : Ty) : Prop :=
+forall (f:fn),
+  DnfFn d f ->
+  forall (v v':V),
+    IsA v (ddom d) ->
+    f v = Res v' ->
+    IsA v' outT ->
+    IsA v inT.
+
+
+Definition overlap (t1 t2:Ty) : bool :=
+  boolean (IsEmpty_dec (tyAnd t1 t2)).
+                 
+
+Definition ainput (a:arrow) (out:Ty) : Ty :=
+  if overlap (rng a) out
+  then (dom a)
+  else emptyTy.
+
+Fixpoint iinput_aux (p: interface) (out:Ty) : Ty :=
+  match p with
+  | IBase a => (ainput a out)
+  | ICons a p' => tyOr (ainput a out) (iinput_aux p' out)
+  end.
+
+Definition iinput (i:interface) (out:Ty) : Ty :=
+  iinput_aux (ipowerset i) out.
 
 (* TODO actual definition *)
-Fixpoint calcIn (f : (V -> res)) (fty:dnf) (t:Ty) : Ty := t. 
+Fixpoint dinput (d:dnf) (out:Ty) : Ty :=
+  match d with
+  | DBase i => iinput i out
+  | DCons i d' => tyOr (iinput i out) (dinput d' out)
+  end. 
 
 
-Theorem calcInSound : forall f t outT inT,
-    TypedDNF f t ->
-    calcIn f t outT = inT ->
-    InputType f outT inT.
+Theorem InputSound : forall d f outT inT,
+    DnfFn d f ->
+    dinput d outT = inT ->
+    DnfInput d inT outT.
 Proof.
   Admitted.
 
 
-Theorem calcInComplete : forall f t outT inT inT',
-    TypedDNF f t ->
-    calcIn f t outT = inT ->
-    InputType f outT inT' ->
+Theorem InputComplete : forall d f outT inT inT',
+    DnfFn d f ->
+    dinput d outT = inT ->
+    DnfInput d inT' outT ->
     Subtype inT inT'.
 Proof.
   Admitted.
